kuiops/common/shmem_aligned/Kuiops.SHMem.CellSend.fst
@@ -1,0 +1,66 @@
+module Kuiops.SHMem.CellSend
+
+#lang-pulse
+
+open Kuiper
+open Kuiper.Array.Vectorized { has_vec_cpy, chunk }
+open Kuiper.Tensor
+open Kuiper.SHMem { is_block_array }
+
+#set-options "--fuel 1 --ifuel 1 --z3rlimit 15"
+
+module FB = Kuiops.GEMM.T.FlipFlopBarrier2
+
+let is_send_across_tensor_cell
+  (#et : Type0) (#r : nat) (#d : shape r)
+  (#l : tlayout d)
+  (a : tensor et l)
+  (vis : visibility)
+  (#_ : squash (visibility_of (core a) == vis))
+  (#f : perm)
+  (i : abs d)
+  (v : et)
+  : is_send_across vis (tensor_pts_to_cell a #f i v)
+=
+  tensor_pts_to_cell_eq a i f v;
+  let idx = l.imap.f i in
+  (* pts_to_cell unfolds to pts_to_slice, which is block/anywhere sendable at
+     the visibility of the backing array. *)
+  let base
+    : is_send_across (visibility_of (core a))
+        (pts_to_cell (core a) #f idx v) = solve in
+  coerce_eq () base
+
+let own_strided_chunks_block_sendable
+  (#et : Type0) {| sized et, has_vec_cpy et |}
+  (#rows #cols : nat)
+  (#l : layout2 rows cols)
+  (m : array2 et l)
+  (#_ : squash (is_block_array (core m)))
+  (em : chest2 et rows cols)
+  (nthr : nat)
+  (tid : natlt nthr)
+  : is_send_across block_of (FB.own_strided_chunks m em nthr tid)
+=
+  is_send_across_forevery
+    #(ij : (natlt rows & natlt cols){
+        Kuiper.Kernel.GEMM.Copy.Vec2.in_chunk (chunk et) rows cols nthr tid ij})
+    (fun ij -> tensor_pts_to_cell m (idx2 ij._1 ij._2) (acc2 em ij._1 ij._2))
+    block_of
+    #(fun ij ->
+        is_send_across_tensor_cell m block_of #_
+          (idx2 ij._1 ij._2) (acc2 em ij._1 ij._2))
+
+let live_strided_chunks_block_sendable
+  (#et : Type0) {| sized et, has_vec_cpy et |}
+  (#rows #cols : nat)
+  (#l : layout2 rows cols)
+  (m : array2 et l)
+  (#_ : squash (is_block_array (core m)))
+  (nthr : nat)
+  (tid : natlt nthr)
+  : is_send_across block_of (FB.live_strided_chunks m nthr tid)
+=
+  is_send_across_exists
+    (fun em -> FB.own_strided_chunks m em nthr tid)
+    #(fun em -> own_strided_chunks_block_sendable m #_ em nthr tid)
